

From equation (7) & (8)

$$\epsilon_{rr} = \frac{2ur}{r} \quad \epsilon_{\theta\theta} = \frac{ur}{r}$$

$$\frac{d}{dr}(r\epsilon_{\theta\theta}) = \epsilon_{rr} \quad \text{--- (11)}$$

compatibility equation

From equations (5) & (11)

{ LEHI Assumptions }

Aside:

$$\therefore \frac{d}{dr} \left( r \frac{ur}{r} \right) = \frac{d}{dr} (ur) = \epsilon_{rr}$$

$$\epsilon_{\theta\theta} = \frac{1}{E} \left[ \sigma_{\theta\theta} - \nu (\sigma_{rr} + \sigma_{zz}) \right] \quad \text{--- (5)}$$

substitute eq (5) into eq (11)

$$\Rightarrow \frac{d}{dr} \left[ r \frac{1}{E} (\sigma_{\theta\theta} - \nu \sigma_{rr} - \nu \sigma_{zz}) \right] = \epsilon_{rr}$$

$$\Rightarrow \frac{1}{E} (\sigma_{\theta\theta} - \nu \sigma_{rr} - \nu \sigma_{zz}) + \frac{r}{E} \left( \frac{d\sigma_{\theta\theta}}{dr} - \nu \frac{d\sigma_{rr}}{dr} - \nu \frac{d\sigma_{zz}}{dr} \right) = \frac{1}{E} (\sigma_{rr} - \nu \sigma_{\theta\theta} - \nu \sigma_{zz})$$

$$r \left( \frac{d\sigma_{\theta\theta}}{dr} - \nu \frac{d\sigma_{rr}}{dr} - \nu \frac{d\sigma_{zz}}{dz} \right) \quad (4)$$

$$= \sigma_{rr} - \nu \sigma_{\theta\theta} - \cancel{\nu \sigma_{rr}} - \sigma_{\theta\theta} + \nu \sigma_{rr} + \cancel{\nu \sigma_{zz}}$$

$$= (1+\nu)\sigma_{rr} - (1+\nu)\sigma_{\theta\theta}$$

$$r \left( \frac{d\sigma_{\theta\theta}}{dr} - \nu \frac{d\sigma_{rr}}{dr} - \nu \frac{d\sigma_{zz}}{dz} \right) = \frac{(\sigma_{rr} - \sigma_{\theta\theta})}{(1+\nu)}$$

{ compatibility equation }  $\rightarrow (2)$

From assumption (4c), we know that axial strain ( $\epsilon_{zz}$ ) is zero or constant

$$\epsilon_{zz} = 0 \Rightarrow \frac{d}{dr}(\epsilon_{zz}) = 0$$

$$\left\{ \begin{array}{l} \text{LEHI Assumption: Equation 6} \\ \epsilon_{zz} = \frac{1}{E} [\sigma_{zz} - \nu(\sigma_{rr} + \sigma_{\theta\theta})] \end{array} \right\}$$

$$\Rightarrow \frac{d}{dr}(\epsilon_{zz}) = 0$$

$$\Rightarrow \frac{d}{dr} \left[ \frac{1}{E} \{ \sigma_{zz} - \nu \sigma_{rr} - \nu \sigma_{\theta\theta} \} \right] = 0$$

$$\Rightarrow \frac{1}{E} \left[ \frac{d\sigma_{zz}}{dr} - \nu \frac{d\sigma_{rr}}{dr} - \nu \frac{d\sigma_{\theta\theta}}{dr} \right] = 0 \quad (5)$$

$$\Rightarrow \boxed{\frac{d\sigma_{zz}}{dr} = \nu \left( \frac{d\sigma_{rr}}{dr} + \frac{d\sigma_{\theta\theta}}{dr} \right)} \rightarrow (13)$$

Recall

$$\boxed{\frac{\partial \sigma_{rr}}{\partial r} + \frac{1}{r} (\sigma_{rr} - \sigma_{\theta\theta}) = 0} \rightarrow (10)$$

Substitute Equation (10) & (13) into Equation (2)

$$\boxed{r \left( \frac{d\sigma_{\theta\theta}}{dr} - \nu \frac{d\sigma_{rr}}{dr} - \nu \frac{d\sigma_{zz}}{dr} \right) = \frac{\sigma_{rr} - \sigma_{\theta\theta}}{(1+\nu)}} \quad \{ \text{compatibility equation} \} \rightarrow (12)$$

$$r \left[ \frac{d\sigma_{\theta\theta}}{dr} - \nu \frac{d\sigma_{rr}}{dr} - \nu \left\{ \nu \left( \frac{d\sigma_{rr}}{dr} + \frac{d\sigma_{\theta\theta}}{dr} \right) \right\} \right]$$

$$= (1+\nu) \left( -\frac{2}{r} \frac{d\sigma_{rr}}{dr} \right)$$

From (13)

⑥

$$\Rightarrow r \frac{d\sigma_{\theta\theta}}{dr} - r v^2 \frac{d\sigma_{rr}}{dr} - r v^2 \frac{d\sigma_{rr}}{dr} - r v^2 \frac{d\sigma_{\theta\theta}}{dr} + r \frac{d\sigma_{rr}}{dr} + r v^2 \frac{d\sigma_{rr}}{dr} = 0$$

$$\Rightarrow \cancel{r} \left( \frac{d\sigma_{\theta\theta}}{dr} - v^2 \frac{d\sigma_{\theta\theta}}{dr} \right) + \cancel{r} \left( \frac{d\sigma_{rr}}{dr} - v^2 \frac{d\sigma_{rr}}{dr} \right) = 0$$

$$\Rightarrow \left( \frac{d\sigma_{\theta\theta}}{dr} + \frac{d\sigma_{rr}}{dr} \right) - v^2 \left( \frac{d\sigma_{\theta\theta}}{dr} + \frac{d\sigma_{rr}}{dr} \right) = 0$$

$$\Rightarrow (1 - v^2) \left( \frac{d\sigma_{\theta\theta}}{dr} + \frac{d\sigma_{rr}}{dr} \right) = 0$$

$$\Rightarrow \boxed{(1 - v^2) \frac{d}{dr} (\sigma_{\theta\theta} + \sigma_{rr}) = 0} \rightarrow \textcircled{14}$$